feat: lemmas for HashMap.alter and .modify  (#6620)
This PR adds lemmas about HashMap.alter and .modify. These lemmas
describe the interaction of alter and modify with the read methods of
the HashMap. The additions affect the HashMap, the DHashMap and their
respective raw versions. Moreover, the raw versions of alter and modify
are defined.

---------

Co-authored-by: Paul Reichert <6992158+datokrat@users.noreply.github.com>

src/Std/Data/HashMap/Raw.lean
@@ -181,6 +181,14 @@ instance [BEq α] [Hashable α] : GetElem? (Raw α β) α β (fun m a => a ∈ m
     (l : List α) : Raw α Unit :=
   ⟨DHashMap.Raw.Const.unitOfList l⟩
 
+@[inline, inherit_doc DHashMap.Raw.Const.alter] def alter [BEq α] [EquivBEq α] [Hashable α]
+    (m : Raw α β) (a : α) (f : Option β → Option β) : Raw α β :=
+  ⟨DHashMap.Raw.Const.alter m.inner a f⟩
+
+@[inline, inherit_doc DHashMap.Raw.Const.modify] def modify [BEq α] [EquivBEq α] [Hashable α]
+    (m : Raw α β) (a : α) (f : β → β) : Raw α β :=
+  ⟨DHashMap.Raw.Const.modify m.inner a f⟩
+
 section Unverified
 
 /-! We currently do not provide lemmas for the functions below. -/
